VerifiedFilter/Grammar/Readme.md
@@ -4,6 +4,6 @@ In this folder we define a [symbolic regular hedge grammar](./Grammar.lean) and 
 We extend regular expression semantics to include [semantics for hedge nodes](./Lang.lean) and define the mapping between regular expression and semantics in [Denote](./Denote.lean).
 
 We implement three algorithms for filtering hedges using symbolic regular hedge grammars:
-* [JSONSchema](./JSONSchema.lean): an algorithm based on [an algorithm applied to JSONSchema](https://www.balisage.net/Proceedings/vol23/html/Holstege01/BalisageVol23-Holstege01.html), that is easy to understand. This includes definitions and proofs of correctness for derive, validate and filter. We also provide [examples](./JSONSchemaExamples.lean).
+* [JSONmembers](./JSONmembers.lean): an algorithm based on [an algorithm applied to JSONSchema](https://www.balisage.net/Proceedings/vol23/html/Holstege01/BalisageVol23-Holstege01.html), that is easy to understand. This includes definitions and proofs of correctness for derive, validate and filter. We also provide [examples](./JSONSchemaExamples.lean).
 * [Katydid](./Katydid.lean): the optimized Katydid algorithm without memoization including definitions and proofs of correctness for derive, validate and filter. We also provide [examples](./KatydidExamples.lean).
 * [Memoize](./Memoize/Readme.md): the optimized Katydid algorithm with memoization including defintions and proofs of correctness for derive, validate and filter.
